---
code: "UMATMIN10001"
subject: "Mathematics"
title: "Linear and Classical Algebra"
semester: 1
year: 2023
fm: 60
time: "2.30"
---

## Group A

###### $3\times4=12$

### 1. Answer any _four_ questions

### (a) If $a$ be a non-zero complex number and $z$ be any complex number, then define $a^z$. What is the principle value of $a^z$?

### (b) Apply Descarte's rule of sign to find the nature of the roots of the equation:

$$
x^4+2x^2+3x-1=0
$$

Given equation:

$$
f(x)=x^4+2x^2+3x-1=0
$$

The above equation is a polynomial of degree $4$. Therefore, there are $4$ roots to the above polynomial.

In order to find the number of positive roots, we have to count the number of sign changes in $f(x)$.

$$
f(x)=x^4+2x^2+3x-1\\
$$

The only sign change is between, $3x$ and $-1$. Therefore, the number of positive roots is $1$.

In order to find the number of negative roots, we have to count the number of sign changes in $f(-x)$.

$$
f(-x)=x^4+2x^2-3x-1
$$

The only sign change is between $2x^2$ and $-3x$. Therefore, the number of negative roots is $1$.

The remaining roots are imaginary roots. Therefore, imaginary roots is $4-1-1=2$.

### (c) Prove that zero is an eigenvalue of a square matrix.

As per Cayley-Hamilton theorem, any square matrix satisfies its characteristic equation $\psi_A(x)$ as follows:

$$
\begin{align*}
  \psi_A(x)=c_0x^n+c_1x^{n-1}+\ldots+c_{n-1}x+c_n=0&&&&&&&&&&(1)
\end{align*}
$$

But for a square matrix $A$, its determinant is: $\det A=0$. And in the characteristic equation $(1)$:

$$
c_n=\det A=0
$$

Therefore, rewriting the characteristic equation, we get:

$$
\psi_A(x)=c_0x^n+c_1x^{n-1}+\ldots+c_{n-1}x=0
$$

In the above equation, $0$ satisfies $\psi_A(x)$, therby making it an eigenvalue.

Hence proved: Zero is an eigenvalue of a square matrix.

### (d) Define consistent system of equations. Show that the following system of linear equations has infinite number of solutions:

$$
x_1+2x_2=674\\
3x_1+6x_2=2022
$$

**Consistent system of equations**: A system of equations for which a solution exists is said to be consistent system of equations. The solution could either be unique, or there might exist an infinite number of solutions, based on the following conditions:

1. $p(A)=p(A|B)=n$
2. $p(A)=p(A|B)<n$

Where,

- $p(A)$ is the rank of coefficient matrix,
- $p(A|B)$ is the rank of augmented matrix, and
- $n$ is the number of unknowns in the system of equations.

Given equations:

$$
x_1+2x_2=674\\
3x_1+6x_2=2022
$$

Creating the augmented matrix:

$$
\begin{align*}
  [A|B]&=\left[\begin{matrix}
    1&2&:&674\\
    3&6&:&2022
  \end{matrix}\right]\\
  &=\left[\begin{matrix}
    1&2&:&674\\
    0&0&:&0
  \end{matrix}\right] &&[\text{By}\ R_2\rightarrow R_2-3R_1]
\end{align*}
$$

The above is the row reduced echelon matrix. Therefore, we can get the following:

- $p(A)=1$
- $p(A|B)=1$
- $n=2$

Since $p(A)=p(A|B)<n$, therefore there exists an infinite number of solutions for the given set of equations.

### (e) Define rank of a matrix. Find the rank of the following matrix:

$$
\left(\begin{matrix}
    1&0&0&0\\
    1&1&0&0\\
    0&0&1&0\\
    0&0&0&1
  \end{matrix}\right)
$$

**Rank of matrix:** Rank of a matrix $A$, is defined to be the greatest positive integer $r$, such that $A$ has atleast one non-zero minor order of $r$. The rank of $A$ is also called the determinant rank of $A$.

Given matrix:

$$
\begin{align*}
  &=\left[\begin{matrix}
    1&0&0&0\\
    1&1&0&0\\
    0&0&1&0\\
    0&0&0&1
  \end{matrix}\right]\\
  &=\left[\begin{matrix}
    1&0&0&0\\
    0&1&0&0\\
    0&0&1&0\\
    0&0&0&1
  \end{matrix}\right]&&[\text{By}\ R_2\rightarrow R_2-R_1]
\end{align*}
$$

The above is the row-reduced echelon form. Therefore the rank of the matrix can be found by counting the number of non-zero rows in the row-reduced echelon form. Rank of the matrix is $4$.

### (f) If $a, b, c, d$ be positive real numbers, then find the minimum value of the following. When does the minimum value occur?

$$
\frac ab+\frac bc+\frac cd+\frac da
$$

---

## Group B

###### $6\times4=24$

### 2. Answer any _four_ questions

### (a) If $\tan\left(i\log\frac{x-iy}{x+iy}\right)=2$, then prove that $x^2-y^2=xy$.

### (b) If $x,y,z$ are positive real numbers and $x+y+z=1$, prove that:

$$
8xyz\le(1-x)(1-y)(1-z)\le\frac8{27}
$$

### (c) Obtain a row echelon matrix which is row equivalent to the following matrix and hence find its rank.

$$
\left(\begin{matrix}
    0&0&2&2&0\\
    1&3&2&4&1\\
    2&6&2&6&2\\
    3&9&1&10&6
  \end{matrix}\right)
$$

The matrix is:

$$
\begin{align*}
  &=\left(\begin{matrix}
    0&0&2&2&0\\
    1&3&2&4&1\\
    2&6&2&6&2\\
    3&9&1&10&6
  \end{matrix}\right)\\
  &=\left(\begin{matrix}
    1&3&2&4&1\\
    0&0&2&2&0\\
    2&6&2&6&2\\
    3&9&1&10&6
  \end{matrix}\right)&&[R_2\leftrightarrow R_1]\\
  &=\left(\begin{matrix}
    1&3&2&4&1\\
    0&0&2&2&0\\
    0&0&-2&-2&0\\
    0&0&-5&-2&3
  \end{matrix}\right)&&[R_3\rightarrow R_3-2R_1,R_4\rightarrow R_4-3R_1]\\
  &=\left(\begin{matrix}
    1&3&2&4&1\\
    0&0&-5&-2&3\\
    0&0&-2&-2&0\\
    0&0&2&2&0
  \end{matrix}\right)&&[R_2\leftrightarrow R_4]\\
  &=\left(\begin{matrix}
    1&3&0&2&1\\
    0&0&-3&0&3\\
    0&0&-2&-2&0\\
    0&0&0&0&0
  \end{matrix}\right)&&[R_4\rightarrow R_4+R_3, R_2\rightarrow R_2-R_3,R_1\rightarrow R_1+R_3]\\
  &=\left(\begin{matrix}
    1&3&0&2&1\\
    0&0&1&0&-1\\
    0&0&1&1&0\\
    0&0&0&0&0
  \end{matrix}\right)&&[R_3\rightarrow -\frac12 R_3, R_2\rightarrow -\frac13 R_2]\\
  &=\left(\begin{matrix}
    1&3&0&2&1\\
    0&0&1&0&-1\\
    0&0&0&1&1\\
    0&0&0&0&0
  \end{matrix}\right)&&[R_3\rightarrow R_3-R_2]\\
  &=\left(\begin{matrix}
    1&3&0&0&-1\\
    0&0&1&0&-1\\
    0&0&0&1&1\\
    0&0&0&0&0
  \end{matrix}\right)&&[R_1\rightarrow R_1-2R_3]\\
\end{align*}
$$

The above is the row reduced echelon form of the matrix. The rank can be found out by counting the number of non-zero rows, which is $3$.

### (d) State Cayley-Hamilton theorem. Use it to find the inverse of the following matrix:

$$
\left(
  \begin{matrix}
    1&-1&0\\
    1&2&-1\\
    3&2&-2
  \end{matrix}
\right)
$$

**Cayley-Hamilton theorem** states that, any square matrix $A$ without exception satisfies its characteristic equation, $\psi_A(x)$, where $x_n$ can be replaced with $A$:

$$
\psi_A(x)=c_0x^n+c_1x^{n-1}+\ldots+c_{n-1}x+c_n=0
$$

Finding the characteristic equation of the above matrix:

$$
\begin{align*}
  &|A-\lambda I_n|=0\\
  \Rightarrow\ &\left|\left[
    \begin{matrix}
      1&-1&0\\
    1&2&-1\\
    3&2&-2
    \end{matrix}
  \right]-\lambda\left[
    \begin{matrix}
      1&0&0\\
      0&1&0\\
      0&0&1
    \end{matrix}
  \right]\right|=0\\
  \Rightarrow\ &\left|
    \begin{matrix}
      1-\lambda&-1&0\\
      1&2-\lambda&-1\\
      3&2&-2-\lambda
    \end{matrix}
  \right|=0\\
  \Rightarrow\ &(1-\lambda)[(2-\lambda)(-2-\lambda)+2]+(-2-\lambda+3)=0\\
  \Rightarrow\ &(1-\lambda)(\lambda^2-2)+(1-\lambda)=0\\
  \Rightarrow\ &(1-\lambda)(\lambda^2-1)=0\\
  \Rightarrow\ &\lambda^2-\lambda^3-1+\lambda=0\\
  \Rightarrow\ &\lambda^3-\lambda^2-\lambda+1=0
\end{align*}
$$

As per Cayley-Hamilton theorem: $\lambda=A$. Therefore,

$$
\begin{align*}
  &A^3-A^2-A+I_n=0\\
  \Rightarrow\ &A^{-1}(A^3-A^2-A+I_n)=0\\
  \Rightarrow\ &A^2-A-I_n+A^{-1}=0\\
  \Rightarrow\ &A^{-1}=A+I_n-A^2\\
  \Rightarrow\ &A^{-1}=\left[
    \begin{matrix}
      1&-1&0\\
      1&2&-1\\
      3&2&-2
    \end{matrix}
  \right]+\left[
    \begin{matrix}
      1&0&0\\
      0&1&0\\
      0&0&1
    \end{matrix}
  \right]-\left[
    \begin{matrix}
      0&-3&1\\
      0&1&0\\
      -1&-3&2
    \end{matrix}
  \right]\\
  \Rightarrow\ &A^{-1}=\left[
    \begin{matrix}
      2&2&-1\\
      1&2&-1\\
      4&5&-3
    \end{matrix}
  \right]
\end{align*}
$$

Therefore, inverse of matrix A is:

$$
A^{-1}=\left[
    \begin{matrix}
      2&2&-1\\
      1&2&-1\\
      4&5&-3
    \end{matrix}
  \right]
$$

### (e) Let $\alpha,\beta,\gamma$ be the roots of the equation $2x^3+3x^2-x-1=0$, find the equation whose roots are

$$
\frac{\beta+\gamma}{\alpha},\frac{\gamma+\alpha}{\beta},\frac{\alpha+\beta}{\gamma}
$$

Given equation:

$$
f(x)=2x^3+3x^2-x-1=0
$$

Let $y=\frac{\beta+\gamma}{\alpha}$

$$
\begin{align*}
  y&=\frac{\beta+\gamma}{\alpha}\\
  \Rightarrow \alpha y&=\beta+\gamma\\
  \Rightarrow \alpha y&=\sum\alpha-\alpha\\
  \Rightarrow \alpha y&=-\frac32-\alpha\\
  \Rightarrow \alpha(y+1)&=-\frac32\\
  \therefore \alpha&=\frac{-3}{2(y+1)}
\end{align*}
$$

Now $\alpha$ is a root of the equation $f(x)$. Therefore:

$$
\begin{align*}
  f(\alpha)&=2\alpha^3+3\alpha^2-\alpha-1=0\\
  &\Rightarrow 2\left(\frac{-3}{2(y+1)}\right)^3+3\left(\frac{-3}{2(y+1)}\right)^2-\left(\frac{-3}{2(y+1)}\right)-1=0\\
  &\Rightarrow\frac{-27}{4(y+1)^3}+\frac{27}{4(y+1)^2}+\frac{3}{2(y+1)}-1=0\\
  &\Rightarrow-27+27(y+1)+6(y+1)^2-4(y+1)^3=0\\
  &\Rightarrow-4y^3-6y^2+27y+2=0\\
  &\Rightarrow4y^3+6y^2-27y-2=0
\end{align*}
$$

Therefore the transformed equation $f(x)'$ is:

$$
f(x)'=4x^3+6x^2-27x-2=0
$$

### (f) Solve by Cardan's method $x^3-3x-1=0$. Hence find $\cos{\frac\pi9}\cos{\frac{7\pi}9}\cos{\frac{13\pi}9}$.

Given equation:

$$
f(x)=x^3-3x-1=0
$$

Let $z=u^{1/3}+v^{1/3}$.

$$
\begin{align*}
  &z=u^{1/3}+v^{1/3}\\
  \Rightarrow\ &z^3=u+v+3u^{1/3}v^{1/3}(u^{1/3}+v^{1/3})\\
  \Rightarrow\ &z^3-3u^{1/3}v^{1/3}z-(u+v)=0&&[\because u^{1/3}+v^{1/3}=z]
\end{align*}
$$

Comparing the above equation with $f(x)$, we get:

- $u^{1/3}v^{1/3}=1\Rightarrow uv=1$, and
- $u+v=1$

Creating a quadratic equation with the above roots:

$$
\begin{align*}
  g(x)&=x^2-(u+v)x+uv=0\\
  &\Rightarrow x^2-x+1=0\\
  &\Rightarrow x=\frac{1\pm\sqrt{-3}}{2}\\
  &\Rightarrow x=\frac12+i\frac{\sqrt3}2,\frac12-i\frac{\sqrt3}2\\
  &\Rightarrow x=\cos{\frac\pi3}+i\sin{\frac\pi3}, \cos{\frac\pi3}-i\sin{\frac\pi3}
\end{align*}
$$

Considering:

$$
\begin{align*}
  u&=\cos{\frac\pi3}+i\sin{\frac\pi3}\\
  \Rightarrow u^{1/3}&=\cos\left(\frac{2k\pi+\pi/3}{3}\right)+i\sin\left(\frac{2k\pi+\pi/3}{3}\right)\\
  &=\cos\left(\frac{6k\pi+\pi}{9}\right)+i\sin\left(\frac{6k\pi+\pi}{9}\right)
\end{align*}
$$

and,

$$
\begin{align*}
  v&=\cos{\frac\pi3}-i\sin{\frac\pi3}\\
  \Rightarrow v^{1/3}&=\cos\left(\frac{2k\pi+\pi/3}{3}\right)-i\sin\left(\frac{2k\pi+\pi/3}{3}\right)\\
  &=\cos\left(\frac{6k\pi+\pi}{9}\right)-i\sin\left(\frac{6k\pi+\pi}{9}\right)
\end{align*}
$$

Now using these to find the roots of the cubic equation are unique for $k=0,1,2$:

For $k=0$:

$$
\begin{align*}
  x_1&=u^{1/3}+v^{1/3}\\
  &=2\cos\frac{\pi}{9}
\end{align*}
$$

For $k=1$:

$$
\begin{align*}
  x_2&=u^{1/3}+v^{1/3}\\
  &=2\cos\frac{7\pi}{9}
\end{align*}
$$

For $k=2$:

$$
\begin{align*}
  x_3&=u^{1/3}+v^{1/3}\\
  &=2\cos\frac{13\pi}{9}
\end{align*}
$$

Therefore, for $f(x)=x^3-3x-1=0$, the roots are:

$$
x=2\cos\frac{\pi}{9},2\cos\frac{7\pi}{9},2\cos\frac{13\pi}{9}
$$

We know for the above cubic equation:

$$
\begin{align*}
  &x_1x_2x_3=-1\\
  \Rightarrow\ &2^3\left(\cos\frac{\pi}{9}\cos\frac{7\pi}{9}\cos\frac{13\pi}{9}\right)1\\
  \therefore\ &\cos\frac{\pi}{9}\cos\frac{7\pi}{9}\cos\frac{13\pi}{9}=\frac{1}{8}
\end{align*}
$$

---

## Group C

###### $6\times2=12$

### 3. Answer any _two_ questions

### (a) (i) State De-Moivre's theorem for integer and rational indices. Use it to prove that

$$
\cos 5\phi=16\cos^5\phi-20\cos^3\phi+5\cos\phi
$$

**De-Moivre's theorem:** When $n$ is a fraction, positive or negative, and $\phi$ is a real number, then $\cos n\phi+i\sin n\phi$ is one of the values of $(\cos n\phi+i\sin n\phi)^n$. As:

$$
(\cos\phi+i\sin\phi)^n=\cos n\phi+i\sin n\phi
$$

Considering $(\cos\phi+i\sin\phi)^5$:

$$
\begin{align*}
  (\cos\phi+i\sin\phi)^5&=\cos^5\phi+\ ^5C_1\cos^4\phi\cdot i\sin\phi+\ ^5C_2\cos^3\phi\cdot i^2\sin^2\phi+\ ^5C_3\cos^2\phi\cdot i^3\sin^3\phi+\ ^5C_4\cos\phi\cdot i^4\sin^4\phi+i^5\sin^5\phi\\
  &=\cos^5\phi+5\cos^4\phi\cdot i\sin\phi-10\cos^3\phi\sin^2\phi-10\cos^2\phi\cdot i\sin^3\theta+5\cos\phi\sin^4\phi+i\sin^5\phi\\
  &=(\cos^5\phi-10\cos^3\sin^2\phi+5\cos\phi\sin^4\phi)+i(5\cos^4\phi\sin\phi-10\cos^2\phi\sin^3\phi+\sin^5\phi)
\end{align*}
$$

But we know: $(\cos\phi+i\sin\phi)^5=\cos5\phi+i\sin5\phi$. Comparing this with the equation above, we get:

$$
\begin{align*}
  \cos5\phi&=\cos^5\phi-10\cos^3\sin^2\phi+5\cos\phi\sin^4\phi\\
  &=\cos^5\phi-10\cos^3\phi(1-\cos^2\phi)+5\cos\phi(1-\cos^2\phi)^2\\
  &=\cos^5\phi-10\cos^3\phi+10\cos^5\phi+5\cos\phi(1+\cos^4\phi-2\cos^2\phi)\\
  &=11\cos^5\phi-10\cos^3\phi+5\cos\phi+5\cos^5\phi-10\cos^3\phi\\
  &=16\cos^5\phi-20\cos^3\phi+5\cos\phi
\end{align*}
$$

Hence proved that:

$$
\cos 5\phi=16\cos^5\phi-20\cos^3\phi+5\cos\phi
$$

### (a) (ii) Find $\text{mod }z$ and $\arg z$ where $z=1+i\tan\frac{3\pi}{5}$.

### (b) (i) Find the eigenvalues and the corresponding eigenvectors of the matrix

$$
\left[
  \begin{matrix}
    2&2&1\\
    1&3&1\\
    1&2&2
  \end{matrix}
\right]
$$

Let the matrix be $A$, as:

$$
\begin{align*}
  A&=\left[
    \begin{matrix}
      2&2&1\\
      1&3&1\\
      1&2&2
    \end{matrix}
  \right]\\
  \Rightarrow\psi_A(x)&=|A-\lambda I_n|=0\\
  &\Rightarrow\left|
    \begin{matrix}
      2-\lambda&2&1\\
      1&3-\lambda&1\\
      1&2&2-\lambda
    \end{matrix}
  \right|=0\\
  &\Rightarrow(2-\lambda)[(3-\lambda)(2-\lambda)-2]-2(2-\lambda-1)+(2-3+\lambda)=0\\
  &\Rightarrow(2-\lambda)(6-5\lambda+\lambda^2-2)-2(1-\lambda)-(1-\lambda)=0\\
  &\Rightarrow(2-\lambda)(\lambda^2-5\lambda+4)-3(1-\lambda)=0\\
  &\Rightarrow2\lambda^2-10\lambda+8-\lambda^3+5\lambda^2-4\lambda-3+3\lambda=0\\
  &\Rightarrow-\lambda^3+7\lambda^2-11\lambda+5=0\\
  &\Rightarrow\lambda^3-7\lambda^2+11\lambda-5=0\\
  &\Rightarrow(\lambda-1)(\lambda^2-6\lambda+5)=0\\
  &\Rightarrow(\lambda-1)(\lambda-1)(\lambda-5)=0\\
  &\therefore \lambda=1,1,5
\end{align*}
$$

Therefore: $\lambda=1,1,5$ are the necessary eigenvalues. Now finding the eigenvectors:

For $\lambda=5$:

$$
\psi_A(5)=|A-5I_n|=\left|
  \begin{matrix}
    -3&2&1\\
    1&-2&1\\
    1&2&-3
  \end{matrix}
\right|
$$

Solving for $x_1,x_2,x_3$:

$$
\begin{align*}
  &\frac{x_1}{\left|
    \begin{matrix}
      -2&1\\
      2&-3
    \end{matrix}
  \right|}=\frac{-x_2}{\left|
    \begin{matrix}
      1&1\\
      1&-3
    \end{matrix}
  \right|}=\frac{x_3}{\left|
    \begin{matrix}
      1&-2\\
      1&2
    \end{matrix}
  \right|}\\
  &=\frac{x_1}{4}=\frac{x_2}{4}=\frac{x_3}{4}\\
  &=x_1=x_2=x_3
\end{align*}
$$

Let $x_1=x_2=x_3=k$:

$$
\therefore \left(
  \begin{matrix}
    x_1\\
    x_2\\
    x_3
  \end{matrix}
\right)_{\lambda=5}=k\left(
  \begin{matrix}
    1\\
    1\\
    1
  \end{matrix}
\right)
$$

For $\lambda=1$:

$$
\begin{align*}
  &Ax=0\\
  \Rightarrow\ &\left[
    \begin{matrix}
      1&2&1\\
      1&2&1\\
      1&2&1
    \end{matrix}
  \right]\left(
    \begin{matrix}
      x_1\\
      x_2\\
      x_3
    \end{matrix}
  \right)=\left(
    \begin{matrix}
      0\\
      0\\
      0
    \end{matrix}
  \right)\\
  \Rightarrow\ &\left[
    \begin{matrix}
      1&2&1\\
      0&0&0\\
      0&0&0
    \end{matrix}
  \right]\left(
    \begin{matrix}
      x_1\\
      x_2\\
      x_3
    \end{matrix}
  \right)=\left(
    \begin{matrix}
      0\\
      0\\
      0
    \end{matrix}
  \right)&&[A:R_2\rightarrow R_2-R_1,R_3\rightarrow R_3-R_1]
\end{align*}
$$

Therefore, we get: $x_1+2x_2+x_3=0$.

Considering through:

- $x_2=0, x_3=k$, we get: $x_1=-k$. Therefore eigenvector:

  $$
    \therefore \left(
      \begin{matrix}
        x_1\\
        x_2\\
        x_3
      \end{matrix}
    \right)_{\lambda=1}=k\left(
      \begin{matrix}
        -1\\
        0\\
        1
      \end{matrix}
    \right)
  $$

- $x_2=k,x_3=0$, we get: $x_1=-2k$. Therefore eigenvector:
  $$
    \therefore \left(
      \begin{matrix}
        x_1\\
        x_2\\
        x_3
      \end{matrix}
    \right)_{\lambda=1}=k\left(
      \begin{matrix}
        -2\\
        1\\
        0
      \end{matrix}
    \right)
  $$

$$
\therefore \left(
  \begin{matrix}
    x_1\\
    x_2\\
    x_3
  \end{matrix}
\right)_{\lambda=1}=k\left(
  \begin{matrix}
    -1\\
    0\\
    1
  \end{matrix}
\right),k\left(
  \begin{matrix}
    -2\\
    1\\
    0
  \end{matrix}
\right)
$$

### (b) (ii) Determine all values of $(1+\sqrt{3}i)^{\frac34}$ and show that their product is 8.

Given complex number is: $(1+\sqrt{3}i)^{\frac34}$. Converting it into trigonometric form:

$$
\begin{align*}
  \Rightarrow(1+\sqrt{3}i)^{\frac34}&=2\left(\cos\frac{\pi}{3}+i\sin\frac{\pi}{3}\right)^{\frac34}\\
  &=8(\cos\pi+i\sin\pi)^{\frac14}\\
  &=\sqrt[4]{8}\left[\cos\left(\frac{2k\pi+\pi}{4}\right)+i\sin\left(\frac{2k\pi+\pi}{4}\right)\right]\\
\end{align*}
$$

The unique roots $z_i$ are found for $k=0,1,2,3$.

For $k=0$:

$$
\begin{align*}
  z_1=\sqrt[4]{8}\left[\cos\frac\pi4+i\sin\frac\pi4\right]=\sqrt[4]{8}\left(\frac{1}{\sqrt2},\frac{1}{\sqrt2}\right)
\end{align*}
$$

For $k=1$:

$$
\begin{align*}
  z_2=\sqrt[4]{8}\left[\cos\frac{3\pi}4+i\sin\frac{3\pi}4\right]=\sqrt[4]{8}\left(-\frac{1}{\sqrt2},\frac{1}{\sqrt2}\right)
\end{align*}
$$

For $k=2$:

$$
\begin{align*}
  z_3=\sqrt[4]{8}\left[\cos\frac{5\pi}4+i\sin\frac{5\pi}4\right]=\sqrt[4]{8}\left(-\frac{1}{\sqrt2},-\frac{1}{\sqrt2}\right)
\end{align*}
$$

For $k=3$:

$$
\begin{align*}
  z_1=\sqrt[4]{8}\left[\cos\frac{7\pi}4+i\sin\frac{7\pi}4\right]=\sqrt[4]{8}\left(\frac{1}{\sqrt2},-\frac{1}{\sqrt2}\right)
\end{align*}
$$

Multiplying the roots, we get:

$$
\begin{align*}
  z_1z_2z_3z_4&=(\sqrt[4]8)^4\left[\left(\frac{1}{\sqrt2},\frac{1}{\sqrt2}\right)\left(-\frac{1}{\sqrt2},\frac{1}{\sqrt2}\right)\left(-\frac{1}{\sqrt2},-\frac{1}{\sqrt2}\right)\left(\frac{1}{\sqrt2},-\frac{1}{\sqrt2}\right)\right]\\
  &=8\left[(-1,0)\left(-\frac{1}{\sqrt2},-\frac{1}{\sqrt2}\right)\left(\frac{1}{\sqrt2},-\frac{1}{\sqrt2}\right)\right]\\
  &=8[(-1,0)(-1,0)]\\
  &=8
\end{align*}
$$

Hence proved, $z_1z_2z_3z_4=8$.

### (c) (i) Solve the system of linear equations given by:

$$
2x+4y+6z+4w=4\\
2x+5y+7z+6w=3\\
2x+3y+5z+2w=5
$$

Forming the augmented matrix:

$$
\begin{align*}
  [A|B]&=\left[
    \begin{matrix}
      2&4&6&4&:&4\\
      2&5&7&6&:&3\\
      2&3&5&2&:&5
    \end{matrix}
  \right]\\
  &=\left[
    \begin{matrix}
      1&2&3&2&:&2\\
      2&5&7&6&:&3\\
      2&3&5&2&:&5
    \end{matrix}
  \right]&&[R_1\rightarrow\frac12 R_1]\\
  &=\left[
    \begin{matrix}
      1&2&3&2&:&2\\
      0&1&1&2&:&-1\\
      0&-1&-1&-2&:&-1
    \end{matrix}
  \right]&&[R_2\rightarrow R_2-2R_1,R_3\rightarrow R_3-2R_1]\\
  &=\left[
    \begin{matrix}
      1&0&1&-2&:&4\\
      0&1&1&2&:&-1\\
      0&0&0&0&:&0
    \end{matrix}
  \right]&&[R_3\rightarrow R_3+R_2,R_1\rightarrow R_1-2R_2]\\
\end{align*}
$$

The above is the row-reduced echelon form of the augmented matrix.

Since, $p[A]=p[A|B]<n$, where $n=3$, therefore there exists an infinite number of solutions for the above set of equations.

Deriving equations from it:

$$
\begin{align*}
  &x+z-2w=4&&&&&&&&&&(1)\\
  &y+z+2w=-1&&&&&&&&&&(2)
\end{align*}
$$

Taking, $z=t_1,w=t_2$, where: $\{t_1,t_2\}\in\R\in[-\infty,+\infty]$.

Substituting the values of $z,w$ in $(1)$, we get:

$$
x=4-t_1+2t_2
$$

Substituting the values of $z,w$ in $(2)$, we get:

$$
y=4-t_1-2t_2
$$

Since all the values $x,y,z,w$ dependes on $t_1,t_2$.

Thereofore: $\{x,y,z,w\}\in\R\in[-\infty,+\infty]$, i.e., an infinite number of solutions.

### (c) (ii) If $A$ and $B$ be invertible matrices of the same order then show that $AB$ is invertible and $(AB)^{-1}=B^{-1}A^{-1}$. Hence show that $(A^{20})^{-1}=(A^{-1})^{20}$.

Considering two $n\times n$ matrices $A$ and $B$.

Since $A$ is invertible, it is non-singular, $A^{-1}$ exists, and $\det A\ne0$. Furthermore by the definition of an inverse, $A^{-1}A=AA^{-1}=I_n$.

Similarly since $B$ is invertible, it is non-singular, $B^{-1}$ exists, and $\det B\ne0$. Furthermore, by the definition of an inverse, $B^{-1}B=BB^{-1}=I_n$.

$$
\det AB=\det A\cdot\det B\ne0
$$

Therefore, $AB$ is a non-singular matrix, and its inverse exists.

Now:

$$
\begin{align*}
  (AB)(B^{-1}A^{-1})&=A(BB^{-1})A^{-1}\\
  &=(AI_n)A^{-1}\\
  &=AA^{-1}\\
  &=I_n
\end{align*}
$$

Similarly:

$$
\begin{align*}
  (B^{-1}A^{-1})(AB)&=B^{-1}(A^{-1}A)B\\
  &=(B^{-1}I_n)B\\
  &=B^{-1}B\\
  &=I_n
\end{align*}
$$

Therefore, we can say:

$$
\begin{align*}
  (B^{-1}A^{-1})(AB)&=I_n\\
  \Rightarrow (B^{-1}A^{-1})&=(AB)^{-1}
\end{align*}
$$

Hence proved: $(AB)^{-1}=B^{-1}A^{-1}$

Now:

$$
\begin{align*}
  A^{20}(A^{-1})^{20}&=(AA^{-1})^20\\
  &=I_n^{20}\\
  &=I_n\\
  \Rightarrow(A^{-1})^{20}&=(A^{20})^{-1}
\end{align*}
$$

Hence proved: $(A^{-1})^{20}=(A^{20})^{-1}$

### (d) (i) If $\alpha,\beta,\gamma$ be the roots of the equation $x^3+qx+1=0$, find the equation whose roots are

$$
\frac\alpha\beta+\frac\beta\alpha,\frac\beta\gamma+\frac\gamma\beta,\frac\gamma\alpha+\frac\alpha\gamma
$$

Given equation:

$$
f(x)=x^3+qx+1=0
$$

Let $y$ be one of the new roots:

$$
\begin{align*}
  y&=\frac\alpha\beta+\frac\beta\alpha\\
  &=\frac{\alpha^2+\beta^2}{\alpha\beta}.\frac\gamma\gamma\\
  &=\frac{\left(\sum\alpha^2-\gamma^2\right)\gamma}{-1}\\
  &=\frac{\left((\sum\alpha)^2-2\sum\alpha\beta-\gamma^2\right)\gamma}{-1}\\
  &=\frac{(-2q-\gamma^2)\gamma}{-1}\\
  &=2q\gamma+\gamma^3\\
  &\Rightarrow2q\gamma+\gamma^3-y=0=y_\gamma
\end{align*}
$$

Performing:

$$
\begin{align*}
  y_\gamma-f(\gamma)&=2q\gamma+\gamma^3-y-\gamma^3-q\gamma-1=0\\
  &\Rightarrow q\gamma-y-1=0\\
  &\Rightarrow \gamma=\frac{y+1}{q}
\end{align*}
$$

Now, $\gamma$ is a root of the above equation:

$$
\begin{align*}
  \therefore f(\gamma)&=\gamma^3+q\gamma+1=0\\
  &\Rightarrow\left(\frac{y+1}{q}\right)^3+q\left(\frac{y+1}{q}\right)+1=0\\
  &\Rightarrow(y+1)^3+q^3(y+1)+q^3=0\\
  &\Rightarrow y^3+3y^2+(q^3+3)y+(2q^3+1)=0
\end{align*}
$$

Therefore the transformed equation for the new roots is:

$$
f(x)=x^3+3x^2+(q^3+3)x+(2q^3+1)=0
$$

### (d) (ii) If $\alpha,\beta,\gamma$ be the roots of the equation $x^3+qx+1=0$, then prove that

- (I) $\sum\alpha^3=-3$
- (II) $\sum\alpha^5=5q$

Given equation:

$$
f(x)=x^3+qx+1=0
$$

From here we can find out that:

- $\sum\alpha=-b/a=0$
- $\sum\alpha\beta=c/a=q$
- $\alpha\beta\gamma=-d/a=-1$
- $\sum\alpha^2=(\sum\alpha)^2-2\sum\alpha\beta=-2q$

(I) To prove: $\sum\alpha^3=-3$

We know: $f(\alpha)=f(\beta)=f(\gamma)=0$, since $\alpha,\beta,\gamma$ are the roots of $f(x)$.

$$
\begin{align*}
  \therefore f(\alpha)+f(\beta)+f(\gamma)&=(\alpha^3+\beta^3+\gamma^3)+q(\alpha+\beta+\gamma)+3=0\\
  &\Rightarrow\sum\alpha^3+q\sum\alpha+3=0\\
  &\Rightarrow\sum\alpha^3=-3&&[\because \sum\alpha=0]
\end{align*}
$$

Hence proved: $\sum\alpha^3=-3$

(II) To prove: $\sum\alpha^5=5q$

Performing the following:

$$
\alpha^2f(\alpha)=\alpha^5+q\alpha^3+\alpha^2=0\\
\beta^2f(\beta)=\beta^5+q\beta^3+\beta^2=0\\
\gamma^2f(\gamma)=\gamma^5+q\gamma^3+\gamma^2=0
$$

$$
\begin{align*}
  \therefore\ &\alpha^2f(\alpha)+\beta^2f(\beta)+\gamma^2f(\gamma)=0\\
  \Rightarrow\ &(\alpha^5+\beta^5+\gamma^5)+q(\alpha^3+\beta^3+\gamma^3)+(\alpha^2+\beta^2+\gamma^2)=0\\
  \Rightarrow\ &\sum\alpha^5+q\sum\alpha^3+\sum\alpha^2=0\\
  \Rightarrow\ &\sum\alpha^5-3q-2q=0&&[\because\sum\alpha^3=-3,\sum\alpha^2=-2q]\\
  \Rightarrow\ &\sum\alpha^5=5q
\end{align*}
$$

Hence proved: $\sum\alpha^5=5q$
